some changes on naming

INDPRO/Basic.lean
@@ -3,27 +3,27 @@ import Lean
 
 section
 universe u
-variable (pre : Type u ) (const : Type u)  (var : Type u) [DecidableEq var] [DecidableEq pre] [DecidableEq const]
+variable (pred_idents : Type u ) (const_idents : Type u)  (var_idents : Type u) [DecidableEq var_idents] [DecidableEq pred_idents] [DecidableEq const_idents]
 /-definition of Constructor, Predicate and their argument type-/
 
 mutual
 inductive γ  where
  | ι  : γ
- | arrow  : κ  ->  γ -> γ
+ | arrow : κ  ->  γ  ->  γ
 deriving Repr, DecidableEq
 
 inductive κ  where
-| arrow : γ -> κ
+| promote : γ -> κ
 deriving Repr, DecidableEq
 
 inductive ρ  where
- | ο : ρ
+ | o : ρ
  | arrow : σ  -> ρ  -> ρ
 deriving Repr, DecidableEq
 
 inductive σ where
- | c_arrow : γ -> σ
- | p_arrow : ρ  -> σ
+ | c_promote : κ -> σ
+ | p_promote : ρ  -> σ
 deriving Repr, DecidableEq
 
 inductive type where
@@ -37,33 +37,37 @@ open type
 def partial_function (a t) := a -> Option t
 def total_function (a t) := a -> t
 
-def TyEnv  := partial_function var type
-def FunEnv := total_function const γ
-def PreEnv := total_function pre ρ
-def extend (pf : partial_function var type) (v : var) (t :type) (v' : var) : Option type :=  if v' = v then some t else pf v'
+def TyEnv  := partial_function var_idents type
+def FunEnv := total_function const_idents γ
+def PreEnv := total_function pred_idents ρ
+def extend_ (pf : partial_function var_idents type) (v : var_idents) (t :type) (v' : var_idents) : Option type :=  if v' = v then some t else pf v'
+def extend (pf : partial_function var_idents type) (v : var_idents) (t :type) : partial_function var_idents type
+| v' => if v' = v then t else pf v'
 /-definition of Terms and type logic-/
-
+def list_extend   : (pf : partial_function var_idents type) -> ( y : List var_idents) -> ( t : List (σ)) -> partial_function var_idents type
+| A , a::as , b :: bs => list_extend (extend var_idents A a (type.Predicate_Arg b)) as bs
+| A , _ , _ => A
 
 inductive Term where
- | P    : pre     ->   Term
- | c    : const   ->   Term
- | Var  : var     ->   Term
- | app  : Term    ->   Term   ->  Term
+ | pred   : pred_idents    ->       Term
+ | const  : const_idents   ->       Term
+ | var    : var_idents     ->       Term
+ | app    : Term    ->   Term   ->  Term
 deriving Repr
 
 mutual
 inductive Goal_formula where
-  | Atomic : Term pre const var-> Goal_formula
+  | Atomic : Term pred_idents const_idents var_idents -> Goal_formula
   | true : Goal_formula
   | GandH : Goal_formula -> Goal_formula -> Goal_formula
-  | exist : var -> Goal_formula -> Goal_formula
+  | exist : var_idents -> Goal_formula -> Goal_formula
 deriving Repr
 
 inductive Definite_formula where
   | CandD : Definite_formula -> Definite_formula -> Definite_formula
   | true  : Definite_formula
-  | nor_any : List (var) -> Goal_formula -> pre -> List (var) -> Definite_formula
-  | cst_any : List (var) -> Goal_formula -> pre -> const -> List (var) -> Definite_formula
+  | nor_any : List (var_idents) -> Goal_formula -> pred_idents -> List (var_idents) -> Definite_formula
+  | cst_any : List (var_idents) -> Goal_formula -> pred_idents -> const_idents -> List (var_idents) -> Definite_formula
 deriving Repr
 
 end
@@ -76,112 +80,166 @@ deriving instance DecidableEq for Definite_formula
 -- infixl:9 " :. " => Term.app
 -- variable(a b : Term pre const var)
 
-inductive term_has_type {fe : FunEnv const } {pi : PreEnv pre} : TyEnv var -> Term pre const var -> type -> Prop where
-| Var {Δ : TyEnv var} {x : var} {τ : type} :
- Δ x = τ -> term_has_type Δ (Term.Var x) τ
+inductive term_has_type {fe : FunEnv const_idents } {pi : PreEnv pred_idents} : TyEnv var_idents -> Term pred_idents const_idents var_idents -> type -> Prop where
+| Var {Δ : TyEnv var_idents} {x : var_idents} {τ : type} :
+ Δ x = τ -> term_has_type Δ (Term.var x) τ
 
-| App_con {Δ : TyEnv var} {s t : Term pre const var} {left:κ} {right: γ}:
+| App_con {Δ : TyEnv var_idents} {s t : Term pred_idents const_idents var_idents} {left:κ} {right: γ}:
   term_has_type Δ (s) (Constructor (γ.arrow left right))
   -> term_has_type Δ t ( Constructor_Arg  left)
-  -> term_has_type Δ (Term.app s t ) (Constructor right)
+  -> term_has_type  Δ (Term.app s t ) (Constructor right)
 
 
-| App_pre {Δ : TyEnv var} {s t : Term pre const var} {left: σ} {right: ρ}:
+| App_pre {Δ : TyEnv var_idents} {s t : Term pred_idents const_idents var_idents} {left: σ} {right: ρ}:
   term_has_type Δ (s) (Predicate (ρ.arrow left right))
-  -> term_has_type Δ t ( Predicate_Arg  left)
-  -> term_has_type Δ (Term.app s t ) (Predicate right)
+  -> term_has_type  Δ t ( Predicate_Arg  left)
+  -> term_has_type  Δ (Term.app s t ) (Predicate right)
 
-| Cst  {Δ : TyEnv var} {c : const} {y : γ} {fe : FunEnv const }:
-  (fe c = y) -> term_has_type Δ (Term.c c) (type.constructor y)
+| Cst  {Δ : TyEnv var_idents}  {c : const_idents} {y : γ} :
+  (fe c = y) -> term_has_type  Δ (Term.const c) (type.Constructor y)
 
-| Cst_arg  {Δ : TyEnv var}   {c : const} {y : Constructor} {x : Con_arg}:
-  term_has_type Δ (Term.c c) (type.constructor y)
- -> term_has_type Δ (Term.c c) (type.con_arg x)
+| Cst_arg  {Δ : TyEnv var_idents}   {c : Term pred_idents const_idents var_idents} {y : γ}:
+  term_has_type  Δ (c) (type.Constructor y)
+ -> term_has_type Δ (c) (type.Constructor_Arg (κ.promote y))
 
+|Pred {Δ : TyEnv var_idents} {pred : pred_idents} {p : ρ} :
+ (pi pred = p) -> term_has_type Δ (Term.pred pred) (type.Predicate p)
+
+|Pred_arg_c  {Δ : TyEnv var_idents}   {c : Term pred_idents const_idents var_idents} {y : γ}:
+  term_has_type Δ (c) (type.Constructor y)
+ -> term_has_type Δ (c) (type.Predicate_Arg (σ.c_promote (κ.promote y)))
+
+|Pred_arg_p  {Δ : TyEnv var_idents}   {c : Term pred_idents const_idents var_idents} {p : ρ}:
+  term_has_type Δ (c) (type.Predicate p)
+ -> term_has_type Δ (c) (type.Predicate_Arg (σ.p_promote p))
+
+
+
+inductive wrong_term_has_type  : TyEnv var_idents -> Term pred_idents const_idents var_idents -> type -> Prop where
+| App_con {Δ : TyEnv var_idents} {s t : Term pred_idents const_idents var_idents} {left:κ} {right: γ}:
+  wrong_term_has_type Δ (s) (Constructor (γ.arrow left right))
+  -> wrong_term_has_type Δ t ( Constructor_Arg  left)
+  -> wrong_term_has_type Δ (Term.app s t ) (Constructor right)
+
+
+| App_pre {Δ : TyEnv var_idents} {s t : Term pred_idents const_idents var_idents} {left: σ} {right: ρ}:
+  wrong_term_has_type Δ (s) (Predicate (ρ.arrow left right))
+  -> wrong_term_has_type Δ t ( Predicate_Arg  left)
+  -> wrong_term_has_type Δ (Term.app s t ) (Predicate right)
+
+| Cst  {Δ : TyEnv var_idents}{fe : FunEnv const_idents } {c : const_idents} {y : γ} :
+  (fe c = y) -> wrong_term_has_type Δ (Term.const c) (type.Constructor y)
+
+| Cst_arg  {Δ : TyEnv var_idents}   {c : Term pred_idents const_idents var_idents} {y : γ}:
+  wrong_term_has_type Δ (c) (type.Constructor y)
+ -> wrong_term_has_type Δ (c) (type.Constructor_Arg (κ.promote y))
+
+
+
+
+
+
+
+
+
+
+
+
+
+
+
+
+
+
+
+inductive Goal_formula_has_type : TyEnv var_idents-> Goal_formula pred_idents const_idents var_idents-> type -> Prop
+  | True  {Δ : TyEnv var_idents} :
+  Goal_formula_has_type  Δ  (Goal_formula.true) (type.Predicate ρ.o)
+
+  | And  {Δ : TyEnv var_idents} {G H: Goal_formula pred_idents const_idents var_idents} :
+  Goal_formula_has_type Δ G (type.Predicate ρ.o)
+  -> Goal_formula_has_type Δ H (type.Predicate ρ.o)
+  -> Goal_formula_has_type Δ (Goal_formula.GandH G H) (type.Predicate ρ.o)
+
+  | Ex {Δ : TyEnv var_idents} {G : Goal_formula pred_idents const_idents var_idents} {x : var_idents} {sigma : σ}:
+  Δ x = Option.none->
+  Goal_formula_has_type (extend_ var_idents Δ x (type.Predicate_Arg sigma)) G (type.Predicate ρ.o) ->
+  Goal_formula_has_type Δ (Goal_formula.exist x G) (type.Predicate ρ.o)
 
 
 -- end
-def single_substitution (T : Term pre const var) (s : Term pre const var) (y : var)  : (Term pre const var) :=
+def term_single_substitution (T : Term pred_idents const_idents var_idents) (s : Term pred_idents const_idents var_idents) (y : var_idents)  : (Term pred_idents const_idents var_idents) :=
     match T with
-    | Var n => if n = y then s else T
-    | app n_1 n_2 => Term.app (single_substitution n_1 s y) (single_substitution n_2 s y)
+    | var n => if n = y then s else T
+    | app n_1 n_2 => Term.app (term_single_substitution n_1 s y) (term_single_substitution n_2 s y)
     | _ => T
 
-def substitutions_Term : (T : Term pre const var) -> (s_bar : List (Term pre  const var)) -> (y_bar : List var) -> (Term pre const var)
+def substitutions_Term : (T : Term pred_idents const_idents var_idents) -> (s_bar : List (Term pred_idents  const_idents var_idents)) -> (y_bar : List var_idents) -> (Term pred_idents const_idents var_idents)
 | T , [] , [] => T
-| T, a::as , b::bs => substitutions_Term (single_substitution pre const var T a b) as bs
+| T, a::as , b::bs => substitutions_Term (term_single_substitution pred_idents const_idents var_idents T a b) as bs
 | T , _ , _ => T
 
 
-
-
-
-def helper : (T : Term pre const var) -> ( V: List var) -> Term pre const var
+def helper : (T : Term pred_idents const_idents var_idents) -> ( V: List var_idents) -> Term pred_idents const_idents var_idents
 | T ,  []   => T
-| T ,  a::as => helper (Term.app T (Term.Var a)) as
+| T ,  a::as => helper (Term.app T (Term.var a)) as
 
-def pre_List_app : (Ps : pre) -> (V : List var) -> Term pre const var
-| Ps , [] =>  Term.P Ps
-| Ps , a::as => helper pre const var (Term.app (Term.P Ps) (Term.Var a)) as
+def pre_List_app : (Ps : pred_idents) -> (V : List var_idents) -> Term pred_idents const_idents var_idents
+| Ps , [] =>  Term.pred Ps
+| Ps , a::as => helper pred_idents const_idents var_idents (Term.app (Term.pred Ps) (Term.var a)) as
 
-def cst_List_app : (cst : const) -> (V : List var) -> Term pre const var
-| Cst , [] =>  Term.c Cst
-| Cst , a::as => helper pre const var (Term.app (Term.c Cst) (Term.Var a)) as
+def cst_List_app : (cst : const_idents) -> (V : List var_idents) -> Term pred_idents const_idents var_idents
+| Cst , [] =>  Term.const Cst
+| Cst , a::as => helper pred_idents const_idents var_idents (Term.app (Term.const Cst) (Term.var a)) as
 
-def single_goal (G : Goal_formula pre const var) (s : Term pre const var) (y : var)  : (Goal_formula pre const var) :=
+def single_goal_sub (G : Goal_formula pred_idents const_idents var_idents) (s : Term pred_idents const_idents var_idents) (y : var_idents)  : (Goal_formula pred_idents const_idents var_idents) :=
     match G with
-    | Goal_formula.Atomic t => Goal_formula.Atomic (single_substitution pre const var t s y)
+    | Goal_formula.Atomic t => Goal_formula.Atomic (term_single_substitution pred_idents const_idents var_idents t s y)
     | Goal_formula.true => Goal_formula.true
-    | Goal_formula.GandH G H => Goal_formula.GandH (single_goal G s y) (single_goal H s y)
-    | Goal_formula.exist x G => Goal_formula.exist x (single_goal G s y)
+    | Goal_formula.GandH G H => Goal_formula.GandH (single_goal_sub G s y) (single_goal_sub H s y)
+    | Goal_formula.exist x G => Goal_formula.exist x (single_goal_sub G s y)
 
-def substitution : (G : Goal_formula pre const var) -> (s_bar : List (Term pre  const var)) -> (y_bar : List var) -> (Goal_formula pre const var)
-| T , [] , [] => T
-| G, a::as , b::bs => substitution (single_goal pre const var G a b) as bs
-| G , _, _  => G
+def substitution : (G : Goal_formula pred_idents const_idents var_idents) -> (s_bar : List (Term pred_idents const_idents var_idents)) -> (y_bar : List var_idents) -> (Goal_formula pred_idents const_idents var_idents)
+| G, a::as , b::bs => substitution (single_goal_sub  pred_idents const_idents var_idents G a b) as bs
+| G , _ , _  => G
 
-def break_ (D : Definite_formula pre const var) :  Prod (Goal_formula pre const var) (Goal_formula pre const var) :=
+def break_ (D : Definite_formula pred_idents const_idents var_idents) :  Prod (Goal_formula pred_idents const_idents var_idents) (Goal_formula pred_idents const_idents var_idents) :=
     match D with
     | Definite_formula.true => (Goal_formula.true , Goal_formula.true)
-    | Definite_formula.nor_any _ G p v => (G , Goal_formula.Atomic (pre_List_app pre const var p v))
-    | Definite_formula.cst_any _ G p cst v =>  (G , Goal_formula.Atomic (Term.app (Term.P p) (cst_List_app pre const var cst v)))
+    | Definite_formula.nor_any _ G p v => (G , Goal_formula.Atomic (pre_List_app pred_idents const_idents var_idents p v))
+    | Definite_formula.cst_any _ G p cst v =>  (G , Goal_formula.Atomic (Term.app (Term.pred p) (cst_List_app pred_idents const_idents var_idents cst v)))
     | Definite_formula.CandD _ _=>  (Goal_formula.true , Goal_formula.true)
-
-
-
-inductive Goal_formula_has_type : TyEnv var-> Goal_formula pre const var-> type -> Prop
-  | True  {Δ : TyEnv var} {G : true } {o : Prop} :
-  Goal_formula_has_type  Δ  (Goal_formula.true) (type.predicate Predicate.o)
-
-  | And  {Δ : TyEnv var} {G H: Goal_formula pre const var} {o : Prop} :
-  Goal_formula_has_type Δ G (type.predicate Predicate.o)
-  -> Goal_formula_has_type Δ H (type.predicate Predicate.o)
-  -> Goal_formula_has_type Δ (Goal_formula.GandH G H) (type.predicate Predicate.o)
-
-  | Ex {Δ : TyEnv var} { new : TyEnv var} {empty : TyEnv var}{G : Goal_formula pre const var} {x : var} {sigma: Pre_arg}:
-  term_has_type pre const var empty (Term.Var x) (type.pre_arg sigma)
-  -> Goal_formula_has_type  Δ  G  (type.predicate Predicate.o)
-  -> Goal_formula_has_type  new  (Goal_formula.exist x G) (type.predicate Predicate.o)
 
   -- | CI {Δ : TyEnv var} { new : TyEnv var} {Ly : List (Term pre const var)} {G : Goal_formula const pre var} {A : Term pre const var} :
   -- term_has_type const pre var Δ Ly
+inductive Definite_formula_has_type : TyEnv var_idents-> Definite_formula pred_idents const_idents var_idents-> type -> Prop
+|CI_nor  {Δ : TyEnv var_idents} {G : Goal_formula pred_idents const_idents var_idents} {y : List var_idents} {t : List σ} {P : pred_idents} :
+Goal_formula_has_type pred_idents const_idents var_idents (list_extend var_idents Δ y t) G (type.Predicate ρ.o) ->
+Goal_formula_has_type pred_idents const_idents var_idents (list_extend var_idents Δ y t) (Goal_formula.Atomic (pre_List_app pred_idents const_idents var_idents P y)) (type.Predicate ρ.o) ->
+Definite_formula_has_type Δ (Definite_formula.nor_any y G P y) (type.Predicate ρ.o)
 
-inductive Prove_Goal_formula: List (Definite_formula pre const var) -> Goal_formula pre const var-> Prop
-| T {D :List (Definite_formula pre const var) } :
+| CI_cst  {Δ : TyEnv var_idents} {G: Goal_formula pred_idents const_idents var_idents} {y : List var_idents} {t : List σ} {P : pred_idents} {con : const_idents} :
+Goal_formula_has_type pred_idents const_idents var_idents (list_extend var_idents Δ y t) G (type.Predicate ρ.o) ->
+Goal_formula_has_type pred_idents const_idents var_idents (list_extend var_idents Δ y t) (Goal_formula.Atomic (Term.app (Term.pred P ) (cst_List_app pred_idents const_idents var_idents con y))) (type.Predicate ρ.o) ->
+Definite_formula_has_type Δ (Definite_formula.cst_any y G P con y) (type.Predicate ρ.o)
+
+inductive Prove_Goal_formula: List (Definite_formula pre_idents const_idents var_idents) -> Goal_formula pred_idents const_idents var_idents-> Prop
+| T {D :List (Definite_formula pred_idents const_idents var_idents) } :
   Prove_Goal_formula D Goal_formula.true
-|And {D :List (Definite_formula pre const var) } {G H :Goal_formula pre const var }:
+|And {D :List (Definite_formula pred_idents const_idents var_idents) } {G H :Goal_formula pred_idents const_idents var_idents }:
   Prove_Goal_formula D G
   -> Prove_Goal_formula D H
   -> Prove_Goal_formula D (Goal_formula.GandH G H)
-| Ex {D :List (Definite_formula pre const var) } (t : Term pre const var) {x : var} {G : Term pre const var}:
-Prove_Goal_formula D (Goal_formula.Atomic (single_substitution pre const var G t x))
--> Prove_Goal_formula D (Goal_formula.exist x (Goal_formula.Atomic G))
 
-| Res {D : List (Definite_formula pre const var)}{ y_bar: List (var)} {s_bar: List (Term pre const var)}{ G A: Goal_formula pre const var} {D_ : Definite_formula pre const var}:
-substitution pre const var (break_ pre const var D_).fst  s_bar y_bar = G  ->
-substitution pre const var (break_ pre const var D_).snd s_bar y_bar = A ->
-Prove_Goal_formula D G->
-Prove_Goal_formula D A
+| Ex {D :List (Definite_formula pred_idents const_idents var_idents) } (t : Term pred_idents const_idents var_idents) {x : var_idents} {G : Goal_formula pred_idents const_idents var_idents}:
+Prove_Goal_formula D ((single_goal_sub pred_idents const_idents var_idents G t x))
+-> Prove_Goal_formula D (Goal_formula.exist x (G))
+
+| Res {D : List (Definite_formula pred_idents const_idents var_idents)}{ y_bar: List (var_idents)} {s_bar: List (Term pred_idents const_idents var_idents)}{ G_ A_: Goal_formula pred_idents const_idents var_idents} {D_ : Definite_formula pred_idents const_idents var_idents}:
+substitution pred_idents const_idents var_idents (break_ pred_idents const_idents var_idents D_).fst  s_bar y_bar = G_  ->
+substitution pred_idents const_idents var_idents (break_ pred_idents const_idents var_idents D_).snd s_bar y_bar = A_ ->
+Prove_Goal_formula D G_->
+Prove_Goal_formula D A_
 
 end
 /- section end-/
@@ -194,13 +252,14 @@ inductive pre_set where
  | Ex : pre_set
  | Open : pre_set
  | Closed : pre_set
+ | Pred : pre_set
 deriving Repr
 
 
 inductive con_set where
  | o : con_set
  | c : con_set
- | bracket : con_set
+ | sqr_bracket : con_set
  | colon : con_set
  | test_txt :con_set
  | ReadMode : con_set
@@ -229,8 +288,8 @@ inductive var_set where
 | h_3: var_set
 | k : var_set
 | y : var_set
+| p : var_set
 deriving Repr
-
 
 deriving instance DecidableEq for pre_set
 deriving instance DecidableEq for con_set
@@ -238,108 +297,113 @@ deriving instance DecidableEq for var_set
 open var_set
 open pre_set
 open con_set
-
-def D_5 : Definite_formula pre_set con_set var_set :=  Definite_formula.cst_any [h,k] (Goal_formula.Atomic (Term.app (Term.P V) (Term.app (Term.Var k) (Term.c o)))) V con_set.open [h,k]
-def D_6 : Definite_formula pre_set con_set var_set :=  Definite_formula.cst_any [h,k] (Goal_formula.Atomic (Term.app (Term.P V) (Term.app (Term.Var k) (Term.c c)))) V con_set.close [h,k]
-def D_7 : Definite_formula pre_set con_set var_set := Definite_formula.cst_any [h, k] (Goal_formula.Atomic (Term.app (Term.P Closed) (Term.Var h))) V con_set.read [h, k]
-def D_10 : Definite_formula pre_set con_set var_set := Definite_formula.cst_any [x, h, k] (Goal_formula.Atomic (Term.app (Term.P V) (Term.app (Term.app (Term.Var x) (Term.Var h)) (Term.app (Term.c putCont) (Term.Var k))))) V con_set.putStrLn [x, h, k]
+def D_1 : Definite_formula pre_set con_set var_set :=  Definite_formula.nor_any [p] (Goal_formula.Atomic (Term.app (Term.var p) (Term.const con_set.sqr_bracket))) pre_set.Ex [p]
+def D_2 : Definite_formula pre_set con_set var_set :=  Definite_formula.nor_any [y,p] (Goal_formula.exist y (Goal_formula.Atomic (Term.app (Term.var p) (Term.app (Term.app (Term.var y) (Term.const con_set.colon)) (Term.const read))))) pre_set.Ex [y, p]
+def D_3 : Definite_formula pre_set con_set var_set :=  Definite_formula.cst_any [x] (Goal_formula.Atomic (Term.app (Term.pred V) (Term.var x))) pre_set.V con_set.id [x]
+def D_4 : Definite_formula pre_set con_set var_set :=  Definite_formula.nor_any [h, k, x] (Goal_formula.Atomic (Term.app (Term.pred V) (Term.app (Term.app (Term.var k) (Term.var x)) (Term.var h)))) pre_set.Pred [h, k ,x ]
+def D_5 : Definite_formula pre_set con_set var_set :=  Definite_formula.cst_any [h,k] (Goal_formula.Atomic (Term.app (Term.pred V) (Term.app (Term.var k) (Term.const o)))) V con_set.open [h,k]
+def D_6 : Definite_formula pre_set con_set var_set :=  Definite_formula.cst_any [h,k] (Goal_formula.Atomic (Term.app (Term.pred V) (Term.app (Term.var k) (Term.const c)))) V con_set.close [h,k]
+def D_7 : Definite_formula pre_set con_set var_set :=  Definite_formula.cst_any [h, k] (Goal_formula.Atomic (Term.app (Term.pred Closed) (Term.var h))) V con_set.read [h, k]
+def D_8 : Definite_formula pre_set con_set var_set :=  Definite_formula.cst_any [h, k] (Goal_formula.GandH (Goal_formula.Atomic (Term.app (Term.pred Open) (Term.var h))) (Goal_formula.Atomic (Term.app (Term.pred Ex) (Term.app (Term.app (Term.pred Pred) (Term.var h)) (Term.var k))))) pre_set.V con_set.read [h,k]
+def D_9 : Definite_formula pre_set con_set var_set :=  Definite_formula.cst_any [k, y, h] (Goal_formula.Atomic (Term.app (Term.pred V) (Term.var k))) V putCont [k,y,h]
+def D_10 : Definite_formula pre_set con_set var_set := Definite_formula.cst_any [x, h, k] (Goal_formula.Atomic (Term.app (Term.pred V) (Term.app (Term.app (Term.var x) (Term.var h)) (Term.app (Term.const putCont) (Term.var k))))) V con_set.putStrLn [x, h, k]
 /- D_11 correspondingt the goal-/
-def D_11 : Definite_formula pre_set con_set var_set := Definite_formula.cst_any [x , m , f , h , k] (Goal_formula.Atomic (Term.app (Term.P V) (Term.app (Term.app (Term.c con_set.open) (Term.Var h)) (Term.app (Term.app (Term.c con_set.withFile_1) (Term.Var f)) (Term.Var k))))) V con_set.withFile [x,m,f,h,k]
-def D_12 : Definite_formula pre_set con_set var_set := Definite_formula.cst_any [f, k ,h_0] (Goal_formula.Atomic (Term.app (Term.P V) (Term.app (Term.app (Term.Var f) (Term.Var h_0)) (Term.app (Term.c con_set.withFile_2) (Term.Var k))))) V con_set.withFile_1 [f, k , h_0]
-def D_13 : Definite_formula pre_set con_set var_set := Definite_formula.cst_any [k, h_1, y] (Goal_formula.Atomic (Term.app (Term.P V) (Term.app (Term.app (Term.c con_set.close) (Term.Var h_1)) (Term.app (Term.app (Term.c con_set.withFile_3) (Term.Var y)) (Term.Var k))))) V con_set.withFile_2 [k, h_1, y]
-def D_14 : Definite_formula pre_set con_set var_set := Definite_formula.cst_any [y, k ,h_2] (Goal_formula.Atomic (Term.app (Term.P V) (Term.app (Term.app (Term.Var k) (Term.Var y)) (Term.Var h_2)))) V con_set.withFile_3 [y, k ,h_2]
-def D_15 : Definite_formula pre_set con_set var_set := Definite_formula.cst_any  [h, k] (Goal_formula.GandH (Goal_formula.Atomic (Term.app (Term.P Open) (Term.Var h))) (Goal_formula.Atomic (Term.app (Term.P V) (Term.app (Term.app (Term.Var k) (Term.c o)) (Term.c con_set.read))))) V con_set.hGetContent [h,k]
-def D_16 : Definite_formula pre_set con_set var_set := Definite_formula.cst_any [x, h_3]  (Goal_formula.Atomic (Term.app (Term.P V ) (Term.app  (Term.app (Term.app (Term.c con_set.putStrLn) (Term.Var var_set.x)) (Term.Var var_set.h_3)) (Term.c id)))) V con_set.act_2 [x, h_3]
+def D_11 : Definite_formula pre_set con_set var_set := Definite_formula.cst_any [x , m , f , h , k] (Goal_formula.Atomic (Term.app (Term.pred V) (Term.app (Term.app (Term.const con_set.open) (Term.var h)) (Term.app (Term.app (Term.const con_set.withFile_1) (Term.var f)) (Term.var k))))) V con_set.withFile [x,m,f,h,k]
+def D_12 : Definite_formula pre_set con_set var_set := Definite_formula.cst_any [f, k ,h_0] (Goal_formula.Atomic (Term.app (Term.pred V) (Term.app (Term.app (Term.var f) (Term.var h_0)) (Term.app (Term.const con_set.withFile_2) (Term.var k))))) V con_set.withFile_1 [f, k , h_0]
+def D_13 : Definite_formula pre_set con_set var_set := Definite_formula.cst_any [k, h_1, y] (Goal_formula.Atomic (Term.app (Term.pred V) (Term.app (Term.app (Term.const con_set.close) (Term.var h_1)) (Term.app (Term.app (Term.const con_set.withFile_3) (Term.var y)) (Term.var k))))) V con_set.withFile_2 [k, h_1, y]
+def D_14 : Definite_formula pre_set con_set var_set := Definite_formula.cst_any [y, k ,h_2] (Goal_formula.Atomic (Term.app (Term.pred V) (Term.app (Term.app (Term.var k) (Term.var y)) (Term.var h_2)))) V con_set.withFile_3 [y, k ,h_2]
+def D_15 : Definite_formula pre_set con_set var_set := Definite_formula.cst_any  [h, k] (Goal_formula.GandH (Goal_formula.Atomic (Term.app (Term.pred Open) (Term.var h))) (Goal_formula.Atomic (Term.app (Term.pred V) (Term.app (Term.app (Term.var k) (Term.const o)) (Term.const con_set.read))))) V con_set.hGetContent [h,k]
+def D_16 : Definite_formula pre_set con_set var_set := Definite_formula.cst_any [x, h_3]  (Goal_formula.Atomic (Term.app (Term.pred V ) (Term.app  (Term.app (Term.app (Term.const con_set.putStrLn) (Term.var var_set.x)) (Term.var var_set.h_3)) (Term.const id)))) V con_set.act_2 [x, h_3]
 def D_17 : Definite_formula pre_set con_set var_set := Definite_formula.cst_any [] Goal_formula.true pre_set.Open con_set.o []
 def D_18 : Definite_formula pre_set con_set var_set := Definite_formula.cst_any [] Goal_formula.true pre_set.Closed con_set.c []
 
 
-def D : List (Definite_formula pre_set con_set var_set) := [D_5, D_6, D_7, D_10, D_11,D_12, D_13, D_14,D_15, D_16,D_17, D_18]
+def D : List (Definite_formula pre_set con_set var_set) := [D_1,D_2,D_3,D_4, D_5, D_6, D_7, D_8, D_9, D_10, D_11,D_12, D_13, D_14,D_15, D_16,D_17, D_18]
 
 theorem base_ : Prove_Goal_formula pre_set con_set var_set D Goal_formula.true :=  Prove_Goal_formula.T
 
-theorem eighteen_ : Prove_Goal_formula pre_set con_set var_set D (Goal_formula.Atomic (Term.app (Term.P Closed) (Term.c c))) :=
-have sub_1: substitution pre_set con_set var_set (break_ pre_set con_set var_set D[11]).fst [] [] = substitution pre_set con_set var_set Goal_formula.true [] []  := by rfl
-have sub_2 : substitution pre_set con_set var_set (break_ pre_set con_set var_set D[11]).snd [] [] =  (Goal_formula.Atomic (Term.app (Term.P Closed) (Term.c c))) := by rfl
+theorem eighteen_ : Prove_Goal_formula pre_set con_set var_set D (Goal_formula.Atomic (Term.app (Term.pred Closed) (Term.const c))) :=
+have sub_1: substitution pre_set con_set var_set (break_ pre_set con_set var_set D[17]).fst [] [] = substitution pre_set con_set var_set Goal_formula.true [] []  := by rfl
+have sub_2 : substitution pre_set con_set var_set (break_ pre_set con_set var_set D[17]).snd [] [] =  (Goal_formula.Atomic (Term.app (Term.pred Closed) (Term.const c))) := by rfl
 Prove_Goal_formula.Res sub_1 sub_2 base_
 
-theorem seven_: Prove_Goal_formula pre_set con_set var_set D  (Goal_formula.Atomic (Term.app (Term.P V ) (Term.app (Term.app (Term.c con_set.read) (Term.c con_set.c)) (Term.app (Term.c con_set.putCont) (Term.c id))))) :=
- have sub_1 : substitution pre_set con_set var_set (break_ pre_set con_set var_set D[2]).fst [(Term.c con_set.c), (Term.app (Term.c con_set.putCont) (Term.c id))] [var_set.h, var_set.k] =
-substitution pre_set con_set var_set (Goal_formula.Atomic (Term.app (Term.P Closed) (Term.c c))) [] []  := by rfl
-have sub_2 : substitution pre_set con_set var_set (break_ pre_set con_set var_set D[2]).snd [(Term.c con_set.c), (Term.app (Term.c con_set.putCont) (Term.c id))] [var_set.h, var_set.k] = (Goal_formula.Atomic (Term.app (Term.P V ) (Term.app (Term.app (Term.c con_set.read) (Term.c con_set.c)) (Term.app (Term.c con_set.putCont) (Term.c id))))) := by rfl
+theorem seven_: Prove_Goal_formula pre_set con_set var_set D  (Goal_formula.Atomic (Term.app (Term.pred V ) (Term.app (Term.app (Term.const con_set.read) (Term.const con_set.c)) (Term.app (Term.const con_set.putCont) (Term.const id))))) :=
+ have sub_1 : substitution pre_set con_set var_set (break_ pre_set con_set var_set D[6]).fst [(Term.const con_set.c), (Term.app (Term.const con_set.putCont) (Term.const id))] [var_set.h, var_set.k] =
+substitution pre_set con_set var_set (Goal_formula.Atomic (Term.app (Term.pred Closed) (Term.const c))) [] []  := by rfl
+have sub_2 : substitution pre_set con_set var_set (break_ pre_set con_set var_set D[6]).snd [(Term.const con_set.c), (Term.app (Term.const con_set.putCont) (Term.const id))] [var_set.h, var_set.k] = (Goal_formula.Atomic (Term.app (Term.pred V ) (Term.app (Term.app (Term.const con_set.read) (Term.const con_set.c)) (Term.app (Term.const con_set.putCont) (Term.const id))))) := by rfl
 Prove_Goal_formula.Res sub_1 sub_2 eighteen_
 
-theorem ten_:Prove_Goal_formula pre_set con_set var_set D (Goal_formula.Atomic (Term.app (Term.P V ) (Term.app (Term.app (Term.app (Term.c con_set.putStrLn) (Term.c con_set.read)) ( Term.c c))  (Term.c id)))) :=
-have sub_1: substitution pre_set con_set var_set (break_ pre_set con_set var_set D[3]).fst [Term.c con_set.read, Term.c c, Term.c id] [x, h, k]=
-(substitution pre_set con_set var_set (Goal_formula.Atomic (Term.app (Term.P V ) (Term.app (Term.app (Term.c con_set.read) (Term.Var var_set.h)) (Term.Var var_set.k))))
-[(Term.c con_set.c), (Term.app (Term.c con_set.putCont) (Term.c id))] [var_set.h, var_set.k]) := by rfl
-have sub_2 : substitution pre_set con_set var_set (break_ pre_set con_set var_set D[3]).snd [Term.c con_set.read, Term.c c, Term.c id] [x, h, k] =
-(Goal_formula.Atomic (Term.app (Term.P V ) (Term.app (Term.app (Term.app (Term.c con_set.putStrLn) (Term.c con_set.read)) ( Term.c c))  (Term.c id)))) := by rfl
+theorem ten_:Prove_Goal_formula pre_set con_set var_set D (Goal_formula.Atomic (Term.app (Term.pred V ) (Term.app (Term.app (Term.app (Term.const con_set.putStrLn) (Term.const con_set.read)) ( Term.const c))  (Term.const id)))) :=
+have sub_1: substitution pre_set con_set var_set (break_ pre_set con_set var_set D[9]).fst [Term.const con_set.read, Term.const c, Term.const id] [x, h, k]=
+(substitution pre_set con_set var_set (Goal_formula.Atomic (Term.app (Term.pred V ) (Term.app (Term.app (Term.const con_set.read) (Term.var var_set.h)) (Term.var var_set.k))))
+[(Term.const con_set.c), (Term.app (Term.const con_set.putCont) (Term.const id))] [var_set.h, var_set.k]) := by rfl
+have sub_2 : substitution pre_set con_set var_set (break_ pre_set con_set var_set D[9]).snd [Term.const con_set.read, Term.const c, Term.const id] [x, h, k] =
+(Goal_formula.Atomic (Term.app (Term.pred V ) (Term.app (Term.app (Term.app (Term.const con_set.putStrLn) (Term.const con_set.read)) ( Term.const c))  (Term.const id)))) := by rfl
 Prove_Goal_formula.Res sub_1 sub_2 seven_
 
-theorem sixteen_ : Prove_Goal_formula pre_set con_set var_set D (Goal_formula.Atomic (Term.app (Term.P V) (Term.app (Term.app (Term.c act_2) (Term.c con_set.read)) (Term.c c))))  :=
-have sub_1 : substitution pre_set con_set var_set (break_ pre_set con_set var_set D[9]).fst [Term.c con_set.read, Term.c con_set.c] [x, h_3] =
-(substitution pre_set con_set var_set (Goal_formula.Atomic (Term.app (Term.P V ) (Term.app (Term.app (Term.app (Term.c con_set.putStrLn) (Term.Var var_set.x)) (Term.Var var_set.h))  (Term.Var k)))) [Term.c con_set.read , Term.c c , Term.c id] [x, h, k])  := by rfl
-have sub_2 : substitution pre_set con_set var_set (break_ pre_set con_set var_set D[9]).snd [Term.c con_set.read, Term.c con_set.c] [x, h_3] =
-(Goal_formula.Atomic (Term.app (Term.P V) (Term.app (Term.app (Term.c act_2) (Term.c con_set.read)) (Term.c c)))) := by rfl
+theorem sixteen_ : Prove_Goal_formula pre_set con_set var_set D (Goal_formula.Atomic (Term.app (Term.pred V) (Term.app (Term.app (Term.const act_2) (Term.const con_set.read)) (Term.const c))))  :=
+have sub_1 : substitution pre_set con_set var_set (break_ pre_set con_set var_set D[15]).fst [Term.const con_set.read, Term.const con_set.c] [x, h_3] =
+(substitution pre_set con_set var_set (Goal_formula.Atomic (Term.app (Term.pred V ) (Term.app (Term.app (Term.app (Term.const con_set.putStrLn) (Term.var var_set.x)) (Term.var var_set.h))  (Term.var k)))) [Term.const con_set.read , Term.const c , Term.const id] [x, h, k])  := by rfl
+have sub_2 : substitution pre_set con_set var_set (break_ pre_set con_set var_set D[15]).snd [Term.const con_set.read, Term.const con_set.c] [x, h_3] =
+(Goal_formula.Atomic (Term.app (Term.pred V) (Term.app (Term.app (Term.const act_2) (Term.const con_set.read)) (Term.const con_set.c)))) := by rfl
 Prove_Goal_formula.Res sub_1 sub_2 ten_
 
 
-theorem fourteen_ : Prove_Goal_formula pre_set con_set var_set D (Goal_formula.Atomic (Term.app (Term.P V) (Term.app (Term.app (Term.app (Term.c con_set.withFile_3) (Term.c con_set.read)) (Term.c act_2)) (Term.c c))))  :=
-have sub_1:  substitution pre_set con_set var_set (break_ pre_set con_set var_set D[7]).fst [Term.c act_2, Term.c con_set.read, Term.c c] [k, y, h_2] =  (substitution pre_set con_set var_set (Goal_formula.Atomic (Term.app (Term.P V) (Term.app (Term.app (Term.c act_2) (Term.Var x)) (Term.Var h_3)))) [Term.c con_set.read, Term.c c] [x, h_3]) := by rfl
-have sub_2 : substitution pre_set con_set var_set (break_ pre_set con_set var_set D[7]).snd [Term.c act_2, Term.c con_set.read, Term.c c] [k, y, h_2] =
-(Goal_formula.Atomic (Term.app (Term.P V) (Term.app (Term.app (Term.app (Term.c con_set.withFile_3) (Term.c con_set.read)) (Term.c act_2)) (Term.c c)))) := by rfl
+theorem fourteen_ : Prove_Goal_formula pre_set con_set var_set D (Goal_formula.Atomic (Term.app (Term.pred V) (Term.app (Term.app (Term.app (Term.const con_set.withFile_3) (Term.const con_set.read)) (Term.const act_2)) (Term.const c))))  :=
+have sub_1:  substitution pre_set con_set var_set (break_ pre_set con_set var_set D[13]).fst [Term.const act_2, Term.const con_set.read, Term.const c] [k, y, h_2] =  (substitution pre_set con_set var_set (Goal_formula.Atomic (Term.app (Term.pred V) (Term.app (Term.app (Term.const act_2) (Term.var x)) (Term.var h_3)))) [Term.const con_set.read, Term.const c] [x, h_3]) := by rfl
+have sub_2 : substitution pre_set con_set var_set (break_ pre_set con_set var_set D[13]).snd [Term.const act_2, Term.const con_set.read, Term.const c] [k, y, h_2] =
+(Goal_formula.Atomic (Term.app (Term.pred V) (Term.app (Term.app (Term.app (Term.const con_set.withFile_3) (Term.const con_set.read)) (Term.const act_2)) (Term.const c)))) := by rfl
 Prove_Goal_formula.Res sub_1 sub_2 sixteen_
 
 
-theorem six_ : Prove_Goal_formula pre_set con_set var_set D  (Goal_formula.Atomic (Term.app (Term.P V) (Term.app (Term.app (Term.c con_set.close) (Term.c o)) ( Term.app (Term.app (Term.c con_set.withFile_3) (Term.c con_set.read)) (Term.c con_set.act_2))))) :=
- have sub_1 : substitution pre_set con_set var_set (break_ pre_set con_set var_set D[1]).fst [Term.c o, Term.app (Term.app (Term.c con_set.withFile_3) (Term.c con_set.read)) (Term.c con_set.act_2)] [h, k] =
- (substitution pre_set con_set var_set (Goal_formula.Atomic (Term.app (Term.P V) (Term.app (Term.app (Term.app (Term.c con_set.withFile_3) (Term.Var y)) (Term.Var k)) (Term.Var h_2)))) [Term.c act_2, Term.c con_set.read, Term.c c] [k, y, h_2] ) := by rfl
-have sub_2 :  substitution pre_set con_set var_set (break_ pre_set con_set var_set D[1]).snd [Term.c o, Term.app (Term.app (Term.c con_set.withFile_3) (Term.c con_set.read)) (Term.c con_set.act_2)] [h, k] =
- (Goal_formula.Atomic (Term.app (Term.P V) (Term.app (Term.app (Term.c con_set.close) (Term.c o)) ( Term.app (Term.app (Term.c con_set.withFile_3) (Term.c con_set.read)) (Term.c con_set.act_2))))) := by rfl
+theorem six_ : Prove_Goal_formula pre_set con_set var_set D  (Goal_formula.Atomic (Term.app (Term.pred V) (Term.app (Term.app (Term.const con_set.close) (Term.const o)) ( Term.app (Term.app (Term.const con_set.withFile_3) (Term.const con_set.read)) (Term.const con_set.act_2))))) :=
+ have sub_1 : substitution pre_set con_set var_set (break_ pre_set con_set var_set D[5]).fst [Term.const o, Term.app (Term.app (Term.const con_set.withFile_3) (Term.const con_set.read)) (Term.const con_set.act_2)] [h, k] =
+ (substitution pre_set con_set var_set (Goal_formula.Atomic (Term.app (Term.pred V) (Term.app (Term.app (Term.app (Term.const con_set.withFile_3) (Term.var y)) (Term.var k)) (Term.var h_2)))) [Term.const act_2, Term.const con_set.read, Term.const c] [k, y, h_2] ) := by rfl
+have sub_2 :  substitution pre_set con_set var_set (break_ pre_set con_set var_set D[5]).snd [Term.const o, Term.app (Term.app (Term.const con_set.withFile_3) (Term.const con_set.read)) (Term.const con_set.act_2)] [h, k] =
+ (Goal_formula.Atomic (Term.app (Term.pred V) (Term.app (Term.app (Term.const con_set.close) (Term.const o)) ( Term.app (Term.app (Term.const con_set.withFile_3) (Term.const con_set.read)) (Term.const con_set.act_2))))) := by rfl
  Prove_Goal_formula.Res sub_1 sub_2 fourteen_
 
 
-theorem thirteen_ : Prove_Goal_formula pre_set con_set var_set D (Goal_formula.Atomic (Term.app (Term.P V) (Term.app ((Term.app ((Term.app (Term.c con_set.withFile_2) (Term.c act_2))) (Term.c o))) (Term.c con_set.read))))  :=
-have sub_1 : substitution pre_set con_set var_set (break_ pre_set con_set var_set D[6]).fst [Term.c act_2, Term.c o, Term.c con_set.read] [k, h_1, y] = (substitution pre_set con_set var_set (Goal_formula.Atomic (Term.app (Term.P V) (Term.app (Term.app (Term.c con_set.close) (Term.Var h)) (Term.Var k))))
- [Term.c o, Term.app (Term.app (Term.c con_set.withFile_3) (Term.c con_set.read)) (Term.c con_set.act_2)] [h, k]) := by rfl
-have sub_2 : substitution pre_set con_set var_set (break_ pre_set con_set var_set D[6]).snd  [Term.c act_2, Term.c o, Term.c con_set.read] [k, h_1 ,y] = (Goal_formula.Atomic (Term.app (Term.P V) (Term.app ((Term.app ((Term.app (Term.c con_set.withFile_2) (Term.c act_2))) (Term.c o))) (Term.c con_set.read)))) := by rfl
+theorem thirteen_ : Prove_Goal_formula pre_set con_set var_set D (Goal_formula.Atomic (Term.app (Term.pred V) (Term.app ((Term.app ((Term.app (Term.const con_set.withFile_2) (Term.const act_2))) (Term.const o))) (Term.const con_set.read))))  :=
+have sub_1 : substitution pre_set con_set var_set (break_ pre_set con_set var_set D[12]).fst [Term.const act_2, Term.const o, Term.const con_set.read] [k, h_1, y] = (substitution pre_set con_set var_set (Goal_formula.Atomic (Term.app (Term.pred V) (Term.app (Term.app (Term.const con_set.close) (Term.var h)) (Term.var k))))
+ [Term.const o, Term.app (Term.app (Term.const con_set.withFile_3) (Term.const con_set.read)) (Term.const con_set.act_2)] [h, k]) := by rfl
+have sub_2 : substitution pre_set con_set var_set (break_ pre_set con_set var_set D[12]).snd  [Term.const act_2, Term.const o, Term.const con_set.read] [k, h_1 ,y] = (Goal_formula.Atomic (Term.app (Term.pred V) (Term.app ((Term.app ((Term.app (Term.const con_set.withFile_2) (Term.const act_2))) (Term.const o))) (Term.const con_set.read)))) := by rfl
 Prove_Goal_formula.Res sub_1 sub_2 six_
 
-theorem seventeen_ : Prove_Goal_formula pre_set con_set var_set D (Goal_formula.Atomic (Term.app (Term.P Open) (Term.c o))) :=
-have sub_1: substitution pre_set con_set var_set (break_ pre_set con_set var_set D[10]).fst [] [] = substitution pre_set con_set var_set Goal_formula.true [] []  := by rfl
-have sub_2 : substitution pre_set con_set var_set (break_ pre_set con_set var_set D[10]).snd [] [] =  (Goal_formula.Atomic (Term.app (Term.P Open) (Term.c o))) := by rfl
+theorem seventeen_ : Prove_Goal_formula pre_set con_set var_set D (Goal_formula.Atomic (Term.app (Term.pred Open) (Term.const o))) :=
+have sub_1: substitution pre_set con_set var_set (break_ pre_set con_set var_set D[16]).fst [] [] = substitution pre_set con_set var_set Goal_formula.true [] []  := by rfl
+have sub_2 : substitution pre_set con_set var_set (break_ pre_set con_set var_set D[16]).snd [] [] =  (Goal_formula.Atomic (Term.app (Term.pred Open) (Term.const o))) := by rfl
 Prove_Goal_formula.Res sub_1 sub_2 base_
 
-theorem combine_ :Prove_Goal_formula pre_set con_set var_set D (Goal_formula.GandH (Goal_formula.Atomic (Term.app (Term.P Open) (Term.c o))) (Goal_formula.Atomic (Term.app (Term.P V) (Term.app ((Term.app ((Term.app (Term.c con_set.withFile_2) (Term.c act_2))) (Term.c o))) (Term.c con_set.read))))) :=
+theorem combine_ :Prove_Goal_formula pre_set con_set var_set D (Goal_formula.GandH (Goal_formula.Atomic (Term.app (Term.pred Open) (Term.const o))) (Goal_formula.Atomic (Term.app (Term.pred V) (Term.app ((Term.app ((Term.app (Term.const con_set.withFile_2) (Term.const act_2))) (Term.const o))) (Term.const con_set.read))))) :=
 Prove_Goal_formula.And seventeen_ thirteen_
 
-theorem fifteen_ : Prove_Goal_formula pre_set con_set var_set D (Goal_formula.Atomic (Term.app (Term.P V) (Term.app (Term.app (Term.c con_set.hGetContent) ( Term.c o)) (Term.app (Term.c con_set.withFile_2) (Term.c act_2))))) :=
-have sub_1 : substitution pre_set con_set var_set (break_ pre_set con_set var_set D[8]).fst [Term.c o, Term.app (Term.c con_set.withFile_2) (Term.c act_2)] [h , k] =
-(@Goal_formula.GandH pre_set con_set var_set (Goal_formula.Atomic (Term.app (Term.P Open) (Term.c o))) (Goal_formula.Atomic (Term.app (Term.P V) (Term.app ((Term.app ((Term.app (Term.c con_set.withFile_2) (Term.c act_2))) (Term.c o))) (Term.c con_set.read))))) := by rfl
-have sub_2 : substitution pre_set con_set var_set (break_ pre_set con_set var_set D[8]).snd [Term.c o, Term.app (Term.c con_set.withFile_2) (Term.c act_2)] [h , k] =
- (Goal_formula.Atomic (Term.app (Term.P V) (Term.app (Term.app (Term.c con_set.hGetContent) ( Term.c o)) (Term.app (Term.c con_set.withFile_2) (Term.c act_2))))) := by rfl
+theorem fifteen_ : Prove_Goal_formula pre_set con_set var_set D (Goal_formula.Atomic (Term.app (Term.pred V) (Term.app (Term.app (Term.const con_set.hGetContent) ( Term.const o)) (Term.app (Term.const con_set.withFile_2) (Term.const act_2))))) :=
+have sub_1 : substitution pre_set con_set var_set (break_ pre_set con_set var_set D[14]).fst [Term.const o, Term.app (Term.const con_set.withFile_2) (Term.const act_2)] [h , k] =
+(@Goal_formula.GandH pre_set con_set var_set (Goal_formula.Atomic (Term.app (Term.pred Open) (Term.const o))) (Goal_formula.Atomic (Term.app (Term.pred V) (Term.app ((Term.app ((Term.app (Term.const con_set.withFile_2) (Term.const act_2))) (Term.const o))) (Term.const con_set.read))))) := by rfl
+have sub_2 : substitution pre_set con_set var_set (break_ pre_set con_set var_set D[14]).snd [Term.const o, Term.app (Term.const con_set.withFile_2) (Term.const act_2)] [h , k] =
+ (Goal_formula.Atomic (Term.app (Term.pred V) (Term.app (Term.app (Term.const con_set.hGetContent) ( Term.const o)) (Term.app (Term.const con_set.withFile_2) (Term.const act_2))))) := by rfl
  Prove_Goal_formula.Res sub_1 sub_2 combine_
 
-theorem twelve_ : Prove_Goal_formula pre_set con_set var_set D (Goal_formula.Atomic (Term.app (Term.P V) (Term.app (Term.app (Term.app (Term.c con_set.withFile_1) ( Term.c con_set.hGetContent)) (Term.c act_2)) (Term.c o)))) :=
-have sub_1 :  substitution pre_set con_set var_set (break_ pre_set con_set var_set D[5]).fst [Term.c con_set.hGetContent, Term.c act_2, Term.c o] [f, k, h_0] =
-(Goal_formula.Atomic (Term.app (Term.P V) (Term.app (Term.app (Term.c con_set.hGetContent) ( Term.c o)) (Term.app (Term.c con_set.withFile_2) (Term.c act_2))))) := by rfl
-have sub_2 : substitution pre_set con_set var_set (break_ pre_set con_set var_set D[5]).snd [Term.c con_set.hGetContent, Term.c act_2, Term.c o] [f, k, h_0] =
-(Goal_formula.Atomic (Term.app (Term.P V) (Term.app (Term.app (Term.app (Term.c con_set.withFile_1) ( Term.c con_set.hGetContent)) (Term.c act_2)) (Term.c o)))) := by rfl
+theorem twelve_ : Prove_Goal_formula pre_set con_set var_set D (Goal_formula.Atomic (Term.app (Term.pred V) (Term.app (Term.app (Term.app (Term.const con_set.withFile_1) ( Term.const con_set.hGetContent)) (Term.const act_2)) (Term.const o)))) :=
+have sub_1 :  substitution pre_set con_set var_set (break_ pre_set con_set var_set D[11]).fst [Term.const con_set.hGetContent, Term.const act_2, Term.const o] [f, k, h_0] =
+(Goal_formula.Atomic (Term.app (Term.pred V) (Term.app (Term.app (Term.const con_set.hGetContent) ( Term.const o)) (Term.app (Term.const con_set.withFile_2) (Term.const act_2))))) := by rfl
+have sub_2 : substitution pre_set con_set var_set (break_ pre_set con_set var_set D[11]).snd [Term.const con_set.hGetContent, Term.const act_2, Term.const o] [f, k, h_0] =
+(Goal_formula.Atomic (Term.app (Term.pred V) (Term.app (Term.app (Term.app (Term.const con_set.withFile_1) ( Term.const con_set.hGetContent)) (Term.const act_2)) (Term.const o)))) := by rfl
 Prove_Goal_formula.Res sub_1 sub_2 fifteen_
 
-theorem five_ : Prove_Goal_formula pre_set con_set var_set D (Goal_formula.Atomic (Term.app (Term.P V) (Term.app (Term.app (Term.c con_set.open) ( Term.c c )) (Term.app (Term.app (Term.c con_set.withFile_1) (Term.c con_set.hGetContent)) (Term.c act_2))))) :=
-have sub_1 : substitution pre_set con_set var_set (break_ pre_set con_set var_set D[0]).fst [Term.c c, Term.app (Term.app (Term.c con_set.withFile_1) (Term.c con_set.hGetContent)) (Term.c act_2)] [h, k] =
-(Goal_formula.Atomic (Term.app (Term.P V) (Term.app (Term.app (Term.app (Term.c con_set.withFile_1) ( Term.c con_set.hGetContent)) (Term.c act_2)) (Term.c o)))) := by rfl
-have sub_2 : substitution pre_set con_set var_set (break_ pre_set con_set var_set D[0]).snd [Term.c c, Term.app (Term.app (Term.c con_set.withFile_1) (Term.c con_set.hGetContent)) (Term.c act_2)] [h, k] =
-(Goal_formula.Atomic (Term.app (Term.P V) (Term.app (Term.app (Term.c con_set.open) ( Term.c c )) (Term.app (Term.app (Term.c con_set.withFile_1) (Term.c con_set.hGetContent)) (Term.c act_2))))) := by rfl
+theorem five_ : Prove_Goal_formula pre_set con_set var_set D (Goal_formula.Atomic (Term.app (Term.pred V) (Term.app (Term.app (Term.const con_set.open) ( Term.const c )) (Term.app (Term.app (Term.const con_set.withFile_1) (Term.const con_set.hGetContent)) (Term.const act_2))))) :=
+have sub_1 : substitution pre_set con_set var_set (break_ pre_set con_set var_set D[4]).fst [Term.const c, Term.app (Term.app (Term.const con_set.withFile_1) (Term.const con_set.hGetContent)) (Term.const act_2)] [h, k] =
+(Goal_formula.Atomic (Term.app (Term.pred V) (Term.app (Term.app (Term.app (Term.const con_set.withFile_1) ( Term.const con_set.hGetContent)) (Term.const act_2)) (Term.const o)))) := by rfl
+have sub_2 : substitution pre_set con_set var_set (break_ pre_set con_set var_set D[4]).snd [Term.const c, Term.app (Term.app (Term.const con_set.withFile_1) (Term.const con_set.hGetContent)) (Term.const act_2)] [h, k] =
+(Goal_formula.Atomic (Term.app (Term.pred V) (Term.app (Term.app (Term.const con_set.open) ( Term.const c )) (Term.app (Term.app (Term.const con_set.withFile_1) (Term.const con_set.hGetContent)) (Term.const act_2))))) := by rfl
 Prove_Goal_formula.Res sub_1 sub_2 twelve_
 
-theorem eleven_ : Prove_Goal_formula pre_set con_set var_set D (Goal_formula.Atomic (Term.app (Term.P V) (Term.app (Term.app (Term.app (Term.app (Term.app (Term.c con_set.withFile) (Term.c con_set.test_txt)) (Term.c con_set.ReadMode)) (Term.c con_set.hGetContent)) (Term.c c)) (Term.c act_2)))) :=
-have sub_1: substitution pre_set con_set var_set (break_ pre_set con_set var_set D[4]).fst [ Term.c con_set.test_txt, Term.c con_set.ReadMode, Term.c con_set.hGetContent, Term.c c, Term.c act_2] [x, m, f, h, k] =
-(Goal_formula.Atomic (Term.app (Term.P V) (Term.app (Term.app (Term.c con_set.open) ( Term.c c )) (Term.app (Term.app (Term.c con_set.withFile_1) (Term.c con_set.hGetContent)) (Term.c act_2))))) := by rfl
-have sub_2: substitution pre_set con_set var_set (break_ pre_set con_set var_set D[4]).snd [ Term.c con_set.test_txt, Term.c con_set.ReadMode, Term.c con_set.hGetContent, Term.c c, Term.c act_2] [x, m, f, h, k] =
-(Goal_formula.Atomic (Term.app (Term.P V) (Term.app (Term.app (Term.app (Term.app (Term.app (Term.c con_set.withFile) (Term.c con_set.test_txt)) (Term.c con_set.ReadMode)) (Term.c con_set.hGetContent)) (Term.c c)) (Term.c act_2)))) := by rfl
+theorem eleven_ : Prove_Goal_formula pre_set con_set var_set D (Goal_formula.Atomic (Term.app (Term.pred V) (Term.app (Term.app (Term.app (Term.app (Term.app (Term.const con_set.withFile) (Term.const con_set.test_txt)) (Term.const con_set.ReadMode)) (Term.const con_set.hGetContent)) (Term.const c)) (Term.const act_2)))) :=
+have sub_1: substitution pre_set con_set var_set (break_ pre_set con_set var_set D[10]).fst [ Term.const con_set.test_txt, Term.const con_set.ReadMode, Term.const con_set.hGetContent, Term.const c, Term.const act_2] [x, m, f, h, k] =
+(Goal_formula.Atomic (Term.app (Term.pred V) (Term.app (Term.app (Term.const con_set.open) ( Term.const c )) (Term.app (Term.app (Term.const con_set.withFile_1) (Term.const con_set.hGetContent)) (Term.const act_2))))) := by rfl
+have sub_2: substitution pre_set con_set var_set (break_ pre_set con_set var_set D[10]).snd [ Term.const con_set.test_txt, Term.const con_set.ReadMode, Term.const con_set.hGetContent, Term.const c, Term.const act_2] [x, m, f, h, k] =
+(Goal_formula.Atomic (Term.app (Term.pred V) (Term.app (Term.app (Term.app (Term.app (Term.app (Term.const con_set.withFile) (Term.const con_set.test_txt)) (Term.const con_set.ReadMode)) (Term.const con_set.hGetContent)) (Term.const c)) (Term.const act_2)))) := by rfl
 Prove_Goal_formula.Res sub_1 sub_2 five_
 
 end LazyIO
@@ -348,47 +412,109 @@ end LazyIO
 namespace simple
  /-con set and pre set-/  /-con set and pre set-/  /-con set and pre set-/  /-con set and pre set-/  /-con set and pre set-/
 inductive con_set where
- | z : con_set
- | s : con_set
-
+ | Z : con_set
+ | S : con_set
 
 inductive pre_set where
- | a : pre_set
+ | Leq : pre_set
 
 inductive var_set where
 |  v : var_set
+
  /-con set and pre set-/  /-con set and pre set-/  /-con set and pre set-/  /-con set and pre set-/  /-con set and pre set-/
 
-def map (x :con_set):=
+def Sigma (x :con_set):=
   match x with
-    | con_set.z => Constructor.individual
-    | con_set.s => Constructor.C  (Con_arg.ctoc Constructor.individual ) Constructor.individual
+    | con_set.Z => γ.ι
+    | con_set.S => γ.arrow  (κ.promote γ.ι ) γ.ι
 
+-- def incorrect_Sigma (x :con_set):=
+--   match x with
+--     | con_set.Z => γ.ι
+--     | con_set.S => γ.ι
 
-def maps (x : pre_set):=
+def Pi (x : pre_set):=
   match x with
-   | pre_set.a => Predicate.o
+   | pre_set.Leq => ρ.arrow (σ.c_promote (κ.promote γ.ι)) (ρ.arrow (σ.c_promote (κ.promote γ.ι)) ρ.o)
 
-
-def mapss (x : var_set)  :=
+def Δ (x : var_set)  :=
   match x with
-    | var_set.v => some (type.constructor Constructor.individual)
+    | var_set.v => some (type.Constructor γ.ι)
+
+deriving instance DecidableEq for pre_set
+deriving instance DecidableEq for con_set
+deriving instance DecidableEq for var_set
+open var_set
+open pre_set
+open con_set
 
 
-variable (z s :const ) (v : var) (TE : TyEnv var_set) (provez : map con_set.z = Constructor.individual) (proves  : map con_set.s = Constructor.C  (Con_arg.ctoc Constructor.individual ) Constructor.individual)
+#check @term_has_type pre_set con_set var_set Sigma Pi Δ
+(Term.app (Term.app (Term.pred pre_set.Leq) (Term.app (Term.const con_set.S) (Term.const con_set.Z))) (Term.const con_set.Z)) (type.Predicate ρ.o)
 
 
-example : @term_has_type pre_set con_set var_set  map  maps mapss (Term.app (Term.c con_set.s) (Term.c con_set.z)) (type.constructor Constructor.individual) :=
-have pz : term_has_type pre_set con_set var_set mapss (Term.c con_set.z) (type.con_arg (Con_arg.ctoc Constructor.individual)) :=
-have sub_pz : term_has_type pre_set con_set var_set mapss (Term.c con_set.z) (type.constructor Constructor.individual) :=
-show term_has_type pre_set con_set var_set mapss (Term.c con_set.z) (type.constructor Constructor.individual) from term_has_type.Cst provez
-show term_has_type pre_set con_set var_set mapss (Term.c con_set.z) (type.con_arg (Con_arg.ctoc Constructor.individual))
-from term_has_type.Cst_arg sub_pz
+theorem Z_ : @term_has_type pre_set con_set var_set Sigma Pi Δ (Term.const Z) (type.Constructor γ.ι) :=
+have sub : Sigma Z = γ.ι := by rfl
+@term_has_type.Cst pre_set con_set var_set Sigma Pi Δ Z γ.ι sub
 
-have ps : term_has_type pre_set con_set var_set mapss (Term.c con_set.s) (type.constructor (Constructor.C  (Con_arg.ctoc Constructor.individual ) Constructor.individual)) :=
-show term_has_type pre_set con_set var_set mapss (Term.c con_set.s) (type.constructor (Constructor.C  (Con_arg.ctoc Constructor.individual ) Constructor.individual))
-from term_has_type.Cst proves
-show @term_has_type pre_set con_set var_set map maps mapss (Term.app (Term.c con_set.s) (Term.c con_set.z)) (type.constructor Constructor.individual) from term_has_type.App_con ps pz
-variable (s : mapss var_set.v = some (type.constructor Constructor.individual))
+theorem Z_con_arg : @term_has_type pre_set con_set var_set Sigma Pi Δ (Term.const Z) (type.Constructor_Arg (κ.promote γ.ι)) := term_has_type.Cst_arg Z_
+theorem Z__pred : @term_has_type pre_set con_set var_set Sigma Pi Δ (Term.const Z) (type.Predicate_Arg (σ.c_promote (κ.promote γ.ι))) := term_has_type.Pred_arg_c Z_
+theorem S_ : @term_has_type pre_set con_set var_set Sigma Pi Δ (Term.const S) (type.Constructor  (γ.arrow  (κ.promote γ.ι ) γ.ι)) :=
+have sub : Sigma S = γ.arrow  (κ.promote γ.ι ) γ.ι := by rfl
+term_has_type.Cst sub
+
+theorem SZ_ : @term_has_type pre_set con_set var_set Sigma Pi Δ (Term.app (Term.const S) (Term.const Z)) (type.Constructor γ.ι) :=
+term_has_type.App_con S_ Z_con_arg
+
+theorem SZ__pred : @term_has_type pre_set con_set var_set Sigma Pi Δ (Term.app (Term.const S) (Term.const Z)) (type.Predicate_Arg (σ.c_promote (κ.promote γ.ι)))
+:= term_has_type.Pred_arg_c SZ_
+
+theorem leq :@term_has_type pre_set con_set var_set Sigma Pi Δ  (Term.pred Leq) (type.Predicate (ρ.arrow (σ.c_promote (κ.promote γ.ι)) (ρ.arrow (σ.c_promote (κ.promote γ.ι)) ρ.o))) :=
+have sub : Pi Leq = ρ.arrow (σ.c_promote (κ.promote  γ.ι)) (ρ.arrow (σ.c_promote (κ.promote γ.ι)) ρ.o) := by rfl
+term_has_type.Pred sub
+
+theorem Leq_SZ : @term_has_type pre_set con_set var_set Sigma Pi Δ  (Term.app (Term.pred Leq) (Term.app (Term.const S) (Term.const Z)))
+ (type.Predicate (ρ.arrow (σ.c_promote (κ.promote γ.ι)) (ρ.o))) := term_has_type.App_pre leq SZ__pred
+theorem Leq_SZ_Z : @term_has_type pre_set con_set var_set Sigma Pi Δ (Term.app (Term.app (Term.pred Leq) (Term.app (Term.const S) (Term.const Z))) (Term.const Z))
+(type.Predicate ρ.o) := term_has_type.App_pre Leq_SZ Z__pred
+
+
+def Leq_SZ_Z_ : Goal_formula pre_set con_set var_set := Goal_formula.Atomic
+(Term.app (Term.app (Term.pred pre_set.Leq) (Term.app (Term.const con_set.S) (Term.const con_set.Z))) (Term.const con_set.Z))
+
+-- theorem Z__ : @term_has_type pre_set con_set var_set incorrect_Sigma Pi Δ (Term.const con_set.Z) (type.Constructor γ.ι) :=
+-- have sub : Sigma con_set.Z = γ.ι := by rfl
+-- term_has_type.Cst  sub
+
+-- -- theorem Z_con_arg : @term_has_type pre_set con_set var_set incorrect_Sigma Pi Δ (Term.const Z) (type.Constructor_Arg (κ.promote γ.ι)) :=
+-- -- term_has_type.Cst_arg Z_
+
+-- theorem S___ : @term_has_type pre_set con_set var_set incorrect_Sigma Pi Δ (Term.const S) (type.Constructor  (γ.arrow  (κ.promote γ.ι ) γ.ι)) :=
+-- have sub : Sigma S = γ.arrow  (κ.promote γ.ι ) γ.ι := by rfl
+-- term_has_type.Cst sub
+
+-- theorem incorrect_SZ : @term_has_type pre_set con_set var_set incorrect_Sigma Pi Δ (Term.app (Term.const S) (Term.const Z)) (type.Constructor γ.ι) :=
+-- term_has_type.App_con S_ Z_con_arg
+
+
+
+-- theorem incorrect_Z : wrong_term_has_type pre_set con_set var_set Δ (Term.const Z) (type.Constructor γ.ι) :=
+-- have sub : incorrect_Sigma Z = γ.ι := by rfl
+-- wrong_term_has_type.Cst  sub
+
+-- theorem incorrect_Z_con_arg : wrong_term_has_type pre_set con_set var_set Δ (Term.const Z) (type.Constructor_Arg (κ.promote γ.ι)) :=
+-- wrong_term_has_type.Cst_arg incorrect_Z
+
+-- theorem incorrect_S : wrong_term_has_type pre_set con_set var_set Δ (Term.const S) (type.Constructor  (γ.arrow  (κ.promote γ.ι ) γ.ι)) :=
+-- have sub : Sigma S = γ.arrow  (κ.promote γ.ι ) γ.ι := by rfl
+-- wrong_term_has_type.Cst sub
+
+-- theorem incorrect_SZ : wrong_term_has_type pre_set con_set var_set Δ (Term.app (Term.const S) (Term.const Z)) (type.Constructor γ.ι) :=
+-- wrong_term_has_type.App_con incorrect_S incorrect_Z_con_arg
+
 
 end simple
+
+
+-- theorem incorrect_SZ_ : wrong_term_has_type  Sigma Pi Δ (Term.app (Term.const S) (Term.const Z)) (type.Constructor γ.ι) :=
+-- have Z_ : wrong_term_has_type
